steel/Zeta.Steel.HashAccumulator.fst
@@ -13,6 +13,7 @@ module R = Steel.ST.Reference
 
 let hash_value_buf  = x:A.array U8.t { A.length x == 32}
 
+[@@CAbstractStruct]
 noeq
 type ha = {
   acc: hash_value_buf;
